bedrock2/src/Semantics.v
@@ -39,9 +39,23 @@ Class parameters := {
 
   mem :> map.map word byte;
   locals :> map.map varname word;
+  env :> map.map funname (list varname * list varname * cmd);
 
   interp_binop : bopname -> word -> word -> word;
-  funname_eqb : funname -> funname -> bool
+  funname_eqb : funname -> funname -> bool;
+
+  trace := list ((mem * actname * list word) * (mem * list word));
+
+  ExtSpec :=
+    (* Given a trace of what happened so far,
+       the current memory, an action label and a list of function call arguments, *)
+    trace -> mem -> actname -> list word ->
+    (* and a postcondition on the new memory and function call results, *)
+    (mem -> list word -> Prop) ->
+    (* tells if this postcondition will hold *)
+    Prop;
+
+  ext_spec: ExtSpec;
 }.
 
 Section semantics.
@@ -52,15 +66,101 @@ Section semantics.
       | access_size.word => Z.to_nat (Z.div (Z.add width 7) 8)
     end%nat.
 
-  Definition trace := list ((mem * actname * list word) * (mem * list word)).
-
-  Definition footprint a sz := List.unfoldn (word.add (word.of_Z 1)) (bytes_per sz) a.
-  Definition load (m:mem) a sz : option word := 
+  Definition footprint(a: word)(sz: access_size) :=
+    List.unfoldn (word.add (word.of_Z 1)) (bytes_per sz) a.
+  Definition load(sz: access_size)(m: mem)(a: word): option word :=
     'Some bs <- List.option_all (List.map (map.get m) (footprint a sz)) | None ;
     Some (word.of_Z (LittleEndian.combine _ (tuple.of_list bs))).
-  Definition unchecked_store (m:mem) a sz v : option mem :=
-    map.putmany_of_list (footprint a sz) (tuple.to_list (LittleEndian.split (bytes_per sz) (word.unsigned v))) m.
-  Definition store sz m a v : option mem :=
-    'Some _ <- load m a sz | None;
-    unchecked_store m a sz v.
+  Definition unchecked_store(sz: access_size)(m: mem)(a: word)(v: word) : option mem :=
+    map.putmany_of_list
+      (footprint a sz)
+      (tuple.to_list (LittleEndian.split (bytes_per sz) (word.unsigned v)))
+      m.
+  Definition store(sz: access_size)(m: mem)(a: word)(v: word): option mem :=
+    'Some _ <- load sz m a | None;
+    unchecked_store sz m a v.
+
+  Implicit Types post : trace -> mem -> locals -> Prop. (* COQBUG(unification finds Type instead of Prop and fails to downgrade *)
+
+  Fixpoint eval_expr(m: mem)(st: locals)(e: expr): option word :=
+    match e with
+    | expr.literal v => Some (word.of_Z v)
+    | expr.var x => map.get st x
+    | expr.load aSize a =>
+        'Some a' <- eval_expr m st a | None;
+        load aSize m a'
+    | expr.op op e1 e2 =>
+        'Some v1 <- eval_expr m st e1 | None;
+        'Some v2 <- eval_expr m st e2 | None;
+        Some (interp_binop op v1 v2)
+    end.
+
+  Section WithEnv.
+    Context (e: env).
+
+    Inductive exec_cmd:
+      cmd ->
+      trace -> mem -> locals ->
+      (trace -> mem -> locals -> Prop) ->
+      Prop :=
+    | ExSkip: forall t m l post,
+        post t m l ->
+        exec_cmd cmd.skip t m l post
+    | ExSet: forall t m l x y y' post,
+        eval_expr m l y = Some y' ->
+        post t m (map.put l x y') ->
+        exec_cmd (cmd.set x y) t m l post
+    | ExStore: forall t m m' l aSize a addr v val post,
+        eval_expr m l a = Some addr ->
+        eval_expr m l v = Some val ->
+        store aSize m addr val = Some m' ->
+        post t m' l ->
+        exec_cmd (cmd.store aSize a v) t m l post
+    | ExIfThen: forall t m l cond vcond bThen bElse post,
+        eval_expr m l cond = Some vcond ->
+        vcond <> word.of_Z 0 ->
+        exec_cmd bThen t m l post ->
+        exec_cmd (cmd.cond cond bThen bElse) t m l post
+    | ExIfElse: forall t m l cond bThen bElse post,
+        eval_expr m l cond = Some (word.of_Z 0) ->
+        exec_cmd bElse t m l post ->
+        exec_cmd (cmd.cond cond bThen bElse) t m l post
+     | ExSeq: forall t m l s1 s2 mid post,
+        exec_cmd s1 t m l mid ->
+        (forall t' m' l', mid t' m' l' -> exec_cmd s2 t' m' l' post) ->
+        exec_cmd (cmd.seq s1 s2) t m l post
+     | ExWhileDone: forall t m l cond body post,
+        eval_expr m l cond = Some (word.of_Z 0) ->
+        post t m l ->
+        exec_cmd (cmd.while cond body) t m l post
+     | ExWhileStep : forall t m l cond body v mid post,
+        eval_expr m l cond  = Some v ->
+        v <> word.of_Z 0 ->
+        exec_cmd body t m l mid ->
+        (forall t' m' l',
+            mid t' m' l' ->
+            exec_cmd (cmd.while cond body) t' m' l' post) ->
+        exec_cmd (cmd.while cond body) t m l post
+     | ExCall: forall t m l binds fname args params rets fbody argvs st0 post outcome,
+        map.get e fname = Some (params, rets, fbody) ->
+        List.option_all (List.map (eval_expr m l) args) = Some argvs ->
+        map.putmany_of_list params argvs map.empty = Some st0 ->
+        exec_cmd fbody t m st0 outcome ->
+        (forall t' m' st1,
+            outcome t' m' st1 ->
+            exists retvs l',
+              List.option_all (List.map (map.get st1) rets) = Some retvs /\
+              map.putmany_of_list binds retvs l = Some l' /\
+              post t' m' l') ->
+        exec_cmd (cmd.call binds fname args) t m l post
+     | ExInteract: forall t m l action argexprs argvals resvars outcome post,
+        List.option_all (List.map (eval_expr m l) argexprs) = Some argvals ->
+        ext_spec t m action argvals outcome ->
+        (forall new_m resvals,
+            outcome new_m resvals ->
+            exists l', map.putmany_of_list resvars resvals l = Some l' /\
+                       post (cons ((m, action, argvals), (new_m, resvals)) t) new_m l') ->
+        exec_cmd (cmd.interact resvars action argexprs) t m l post
+    .
+  End WithEnv.
 End semantics.
